Lean2Js/Builder.lean
@@ -63,6 +63,8 @@ def arrayReverse (arr : Expr) : Expr := .arrayReverse arr
 def map' (arr : Expr) (binder : String) (body : Expr) : Expr := .mapE arr binder body
 def filter' (arr : Expr) (binder : String) (body : Expr) : Expr := .filterE arr binder body
 
+def sortByKey' (arr : Expr) (binder : String) (body : Expr) : Expr := .sortByKeyE arr binder body
+
 def find' (arr : Expr) (binder : String) (body : Expr) : Expr := .findE arr binder body
 def all' (arr : Expr) (binder : String) (body : Expr) : Expr := .quantE .all arr binder body
 def any' (arr : Expr) (binder : String) (body : Expr) : Expr := .quantE .any arr binder body
